src/tutorial/Example3.v
@@ -1,0 +1,134 @@
+From sflib Require Import sflib.
+From Paco Require Import paco.
+From Tutorial Require Import Refinement.
+From Coq Require Import Strings.String List.
+From Tutorial Require Import Imp Simulation.
+
+Set Implicit Arguments.
+
+Section EX.
+  (** Let us revisit examples in Example2.v, and prove them with correct simulation. *)
+
+  (* DIV2. Prove by coinduction. *)
+  Definition src6 : com :=
+    <{ "x" := 100;
+       while ("x")
+       do ("x" := AAny)
+       end;
+       ret "x"
+    }>.
+
+  Definition tgt6 : com :=
+    <{ "x" := 100;
+       while ("x")
+       do ("x" := AAny)
+       end;
+       ret "x"
+    }>.
+
+  (* Solves tgt undef case if tgt is not undef. *)
+  Ltac solve_tgt_ub := 
+    exfalso;
+    match goal with
+    | [UNDEF : forall _ _, ~ (ceval _ _ _) |- _] => eapply UNDEF
+    end;
+    repeat econs.
+
+  (* Makes a tgt step. *)
+  Ltac step_tgt_silent0 :=
+    match goal with
+    | [STEP: ceval _ _ _ |- _] => inv STEP
+    end;
+    ss; split; auto.
+
+  (* Combines above two tactics. *)
+  Ltac step_tgt_silent :=
+    try (guclo @sim_indC_spec; econs 4;
+         [ss
+         | ss; intros ev st_tgt1 STEP0; inv STEP0;
+           [step_tgt_silent0 | solve_tgt_ub]
+        ]).
+
+  (* Makes a src silent step. *)
+  Ltac step_src_silent :=
+    try (guclo @sim_indC_spec; econs 3;
+         [ss
+         | ss; exists (inr LInternal); eexists; splits; ss; [repeat econs | ]
+        ]).
+
+  Goal refines (Imp_Program_Ext src6) (Imp_Program_Ext tgt6).
+  Proof.
+    apply adequacy. unfold simulation, Imp_Program_Ext, Imp_STS_Ext, src6, tgt6, Imp_init.
+    ss. intros.
+    (* *gpaco* is more convenient here: we will do up-to reasoning with the inductive closure (sim_indC). *)
+    ginit.
+    guclo @sim_indC_spec. econs 4. ss.
+    i. inv H. 2: solve_tgt_ub. inv STEP. split; auto.
+    (* Combining above into a tactic and take steps until the while loop. *)
+    step_tgt_silent. step_tgt_silent. step_tgt_silent.
+    inv H6.
+    (* The target reached a while loop. We take the source side to the loop too. *)
+    do 4 step_src_silent.
+    (** Now we start a coinductive proof. We first set up a coinductive hypothesis. *)
+    clear ps pt.
+    remember Reg.init as reg. clear Heqreg.
+    remember 100 as n. clear Heqn.
+    (* Generalize the progress flags. *)
+    pose proof true as ps. pose proof true as pt.
+    guclo @sim_progressC_spec. econs. instantiate (1:=pt). instantiate (1:=ps). 2,3: ss.
+    revert reg n ps pt. gcofix CIH. i.
+    (* Then make progress. *)
+    step_tgt_silent.
+    - (* False case; loop terminates. *)
+      clear CIH.
+      inv H6. inv H1.
+      do 2 step_src_silent.
+      do 2 step_tgt_silent.
+      inv H5. inv H1.
+      do 1 step_src_silent.
+      gstep. econs; ss.
+    - (* True case; loops. *)
+      rename H7 into TRUE. inv H6. inv H1.
+      step_tgt_silent.
+      inv H6.
+      step_tgt_silent.
+      (* Tactic 'step_src_silent' picks wrong constructor, so we prove manually. *)
+      guclo @sim_indC_spec. econs 3; ss. do 2 eexists. splits.
+      { econs 1. eapply E_WhileTrue. repeat econs. auto. }
+      { ss. }
+      (* AAny introduces nondeterminism. We picks what we need when AAny is in the src. *)
+      guclo @sim_indC_spec. econs 3; ss. do 2 eexists. splits.
+      { econs 1. eapply E_Asgn. eapply (E_AAny _ n). }
+      { ss. }
+      step_src_silent.
+      (* Now we came back to the start of the while loop. We can end the proof by coinduction. *)
+      gstep. eapply sim_progress. 2,3: auto.
+      gfinal. left. eapply CIH.
+      Unshelve. exact 0.
+    - (* Leftover undef case. *)
+      exfalso. destruct (Nat.eqb n 0) eqn:CASES.
+      + eapply UNDEF. eapply E_WhileFalse. repeat econs. apply PeanoNat.Nat.eqb_eq. auto.
+      + eapply UNDEF. eapply E_WhileTrue. repeat econs. apply PeanoNat.Nat.eqb_neq; auto.
+  Qed.
+
+
+  (** This simulation is sound, as proven by the adequacy theorem, and the following examples cannot be proven as expected. 
+      You can check that you cannot *unguard* the coinductive hypothesis, because either the source or the target side progress flag is not set to true.
+   *)
+
+  (* EX1. The src terminates, but the tgt diverges. *)
+  Definition src1 : com :=
+    <{ ret 0 }>.
+
+  Definition tgt1 : com :=
+    <{ while (1)
+       do skip
+       end;
+       ret 1
+    }>.
+
+  Goal refines (Imp_Program_Ext src1) (Imp_Program_Ext tgt1).
+  Proof.
+  Admitted.
+
+End EX.
